proof/correctness/Correctness_WOTS.ec
@@ -28,9 +28,9 @@ op load_sig (mem : global_mem_t) (ptr : W64.t) : W8.t Array2144.t =
 (** -------------------------------------------------------------------------------------------- **)
 
 lemma nbyte_xor_val (a b : nbytes): 
-    val (nbytexor a b) = bytexor (val a) (val b).
+    NBytes.val (nbytexor a b) = bytexor (NBytes.val a) (NBytes.val b).
 proof.
-rewrite /nbytexor NBytes.insubdK //= /P /bytexor size_map size_zip !valP //.
+rewrite /nbytexor NBytes.insubdK //= /P /bytexor size_map size_zip !NBytes.valP //.
 qed.
 
 (** -------------------------------------------------------------------------------------------- **)
@@ -314,11 +314,11 @@ conseq (: _ ==>
 ).
   + auto => /> H0 addrL outseedsL skR H1 H2 H3.
     rewrite /DecodeWotsSk tP => j?. 
-    by rewrite get_of_list //= insubdK /P // H2.
+    by rewrite get_of_list //= LenNBytes.insubdK /P // H2.
 
 seq 5 3 : (
-  val sk_seed{2} = to_list inseed{1} /\
-  val seed{2} = to_list pub_seed{1} /\
+  NBytes.val sk_seed{2} = to_list inseed{1} /\
+  NBytes.val seed{2} = to_list pub_seed{1} /\
   size sk{2} = len /\ 
   size (nbytes_flatten sk{2}) = len * n /\
   sub addr{1} 0 5 = sub a1 0 5 /\
@@ -353,8 +353,8 @@ while (
   len{2} = 67 /\
   size sk{2} = len /\ 
   ={i} /\ 0 <= i{2} <= 67 /\ 
-  val sk_seed{2} = to_list inseed{1} /\
-  val seed{2} = to_list pub_seed{1} /\
+  NBytes.val sk_seed{2} = to_list inseed{1} /\
+  NBytes.val seed{2} = to_list pub_seed{1} /\
   sub addr{1} 0 5 = sub a1 0 5 /\
   (forall (k : int), 0 <= k < 32 => buf{1}.[k] = pub_seed{1}.[k]) /\
   (forall (k : int), 0 <= k < 32 * i{2} => outseeds{1}.[k] = nth witness (nbytes_flatten sk{2}) k) /\
@@ -377,7 +377,7 @@ seq 2 1 : (
            case (k = 5) => [->|?] //.
            by rewrite !get_setE // !ifF // H.
  
-seq 1 1 : (#pre /\ val addr_bytes{2} = to_list addr_bytes{1}).
+seq 1 1 : (#pre /\ NBytes.val addr_bytes{2} = to_list addr_bytes{1}).
 - exists * addr{1}; elim * => P.
   call {1} (addr_to_bytes_correctness P).
   auto => /> ??????????????->.
@@ -387,8 +387,8 @@ seq 1 1 : (#pre /\ val addr_bytes{2} = to_list addr_bytes{1}).
           auto => />.
           rewrite (nth_map witness) /=; first by rewrite size_to_list /#.
           by rewrite size_rev size_to_list.
-      rewrite big_constz count_predT size_map size_to_list valP /#.
-  rewrite valP n_val => j?.
+      rewrite big_constz count_predT size_map size_to_list NBytes.valP /#.
+  rewrite NBytes.valP n_val => j?.
   rewrite (nth_flatten witness 4).
     + pose X := (fun (s : W8.t list) => size s = 4).
       pose Y := (map W32toBytes (to_list P)).
@@ -396,7 +396,7 @@ seq 1 1 : (#pre /\ val addr_bytes{2} = to_list addr_bytes{1}).
       by rewrite (nth_map witness) //= size_rev size_to_list.      
   rewrite (nth_map witness); first by rewrite size_to_list /#.
   rewrite /addr_to_bytes => />.
-  rewrite insubdK.
+  rewrite NBytes.insubdK.
     + rewrite /P size_flatten sumzE BIA.big_map /(\o) //= -(StdBigop.Bigint.BIA.eq_big_seq (fun _ => 4)) /=.   
         * rewrite in_nth size_map size_to_list => k?.
           auto => />.
@@ -416,17 +416,17 @@ seq 1 0 : (#pre /\ (forall (k : int), 0 <= k < 32 => buf{1}.[32 + k] = addr_byte
 
 seq 0 0 : ( (* cant use #pre in conseq *)
   #pre /\ 
-  to_list buf{1} = (val seed{2} ++ val addr_bytes{2})
+  to_list buf{1} = (NBytes.val seed{2} ++ NBytes.val addr_bytes{2})
 ).
     + skip => /> &1 &2 ????? H ????? H1 *. 
-      apply (eq_from_nth witness); [by rewrite size_cat H !size_to_list valP n_val |].
+      apply (eq_from_nth witness); [by rewrite size_cat H !size_to_list NBytes.valP n_val |].
       rewrite size_to_list => j Hj.
       rewrite get_to_list.
       case (0 <= j < 32) => *.
         * rewrite nth_cat H size_to_list ifT 1:/# get_to_list /#.
       rewrite nth_cat H size_to_list ifF 1:/# H1 get_to_list /#. 
 
-seq 2 1 : (#pre /\ val sk_i{2} = to_list ith_seed{1}).
+seq 2 1 : (#pre /\ NBytes.val sk_i{2} = to_list ith_seed{1}).
     + inline {1} M(Syscall).__prf_keygen_ M(Syscall)._prf_keygen; wp; sp.
       exists * in_00{1}, key0{1}; elim * => _P1 _P2.
       call {1} (prf_keygen_correctness _P1 _P2) => [/# |].
@@ -477,8 +477,8 @@ proc => /=.
 seq 1 1 : (#pre /\ size pk{2} = len); first by auto => />; rewrite size_nseq /#.
 swap {2} 1 1.
 seq 1 1: (   
-  val sk_seed{2} = to_list seed{1} /\
-  val _seed{2} = to_list pub_seed{1} /\
+  NBytes.val sk_seed{2} = to_list seed{1} /\
+  NBytes.val _seed{2} = to_list pub_seed{1} /\
   pk{1} = DecodeWotsSk wots_skey{2} /\
   size pk{2} = len /\
   sub a1 0 5 = sub a2 0 5 /\
@@ -489,7 +489,7 @@ seq 1 1: (
       wp; sp.
       exists * inseed0{1}, pub_seed1{1}, addr1{1}, address{2}; elim * => _P1 _P2 _P3 _P4.
       call (expand_seed_correct _P1 _P2 _P3 _P4) => [/# |]. 
-      skip => /> &1 &2 *; do split; [| | smt()]; by rewrite insubdK // /P size_to_list n_val.
+      skip => /> &1 &2 *; do split; [| | smt()]; by rewrite NBytes.insubdK // /P size_to_list n_val.
      
 conseq (: _ ==> 
   size pk{2} = len /\
@@ -499,12 +499,12 @@ conseq (: _ ==>
     + auto => /> &1 &2 ??????????*.
       rewrite /DecodeWotsPk tP => j Hj.
       rewrite /of_list initE ifT //=. 
-      by rewrite insubdK /#.
+      by rewrite LenNBytes.insubdK /#.
  
 conseq /> => [/# |].
 while (
-  val sk_seed{2} = to_list seed{1} /\ 
-  val _seed{2} = to_list pub_seed{1} /\
+  NBytes.val sk_seed{2} = to_list seed{1} /\ 
+  NBytes.val _seed{2} = to_list pub_seed{1} /\
   sub address{2} 0 5 = sub addr{1} 0 5 /\
 
   size pk{2} = len /\
@@ -514,7 +514,7 @@ while (
   sub addr{1} 0 5 = sub a1 0 5 /\
 
   (forall (k : int), 0 <= k < 32 * i{1} => pk{1}.[k] = nth witness (nbytes_flatten pk{2}) k) /\
-  (forall (k : int), 32 * i{1} <= k < 2144 => pk{1}.[k] = nth witness (nbytes_flatten (val wots_skey{2})) k)
+  (forall (k : int), 32 * i{1} <= k < 2144 => pk{1}.[k] = nth witness (nbytes_flatten (LenNBytes.val wots_skey{2})) k)
 ); last first.
     + auto => /> &1 &2 H0 H1 H2 H3 H4 H5.
       do split; 1,2,4,5: by smt().
@@ -532,7 +532,7 @@ seq 2 1 : (#pre /\ sub address{2} 0 6 = sub addr{1} 0 6).
         * rewrite ifF 1:/#; smt(sub_k).
         * case (j = 5) => //; smt(sub_k).
  
-seq 2 2 : (#pre /\ to_list t{1} = val pk_i{2}).
+seq 2 2 : (#pre /\ to_list t{1} = NBytes.val pk_i{2}).
     + inline M(Syscall).__gen_chain_inplace_ M(Syscall)._gen_chain_inplace; wp; sp.  
       exists * out0{1}, start0{1}, steps0{1}, pub_seed1{1}, addr1{1}, address{2}.  
       elim * => _P1 _P2 _P3 _P4 _P5 _P6.  
@@ -540,13 +540,13 @@ seq 2 2 : (#pre /\ to_list t{1} = val pk_i{2}).
       skip => /> &1 &2 H0 H1 H2 H3 H4 H5 H6 H7 H8 H9 H10 H11.   
       do split.
           * apply nbytes_eq.
-            rewrite insubdK; [by rewrite /P size_to_list n_val |].
-            apply (eq_from_nth witness); first by rewrite valP n_val size_to_list.
-            rewrite valP n_val => j?.
+            rewrite NBytes.insubdK; [by rewrite /P size_to_list n_val |].
+            apply (eq_from_nth witness); first by rewrite NBytes.valP n_val size_to_list.
+            rewrite NBytes.valP n_val => j?.
             rewrite get_to_list initiE // => />.
             rewrite /nbytes_flatten in H6.
             rewrite H8 1:/#.
-            rewrite nth_nbytes_flatten; first by rewrite valP /#.
+            rewrite nth_nbytes_flatten; first by rewrite LenNBytes.valP /#.
             by do congr => /#. 
           * by rewrite w_val.
           * rewrite -H1 #smt:(@NBytes).  
@@ -566,8 +566,8 @@ auto => /> &1 &2 H0 H1 H2 H3 H4 H5 H6 H7 H8 H9 H10 H11 H12*; do split;2,3,6,7:sm
             rewrite nth_put 1:/# ifF 1:/#.
             rewrite H7 1:/# nth_nbytes_flatten /#.
     + move => k??.
-      rewrite nth_nbytes_flatten; first by rewrite valP /#.
-      by rewrite initiE 1:/# /= ifF 1:/# H8 1:/# nth_nbytes_flatten // valP /#.
+      rewrite nth_nbytes_flatten; first by rewrite LenNBytes.valP /#.
+      by rewrite initiE 1:/# /= ifF 1:/# H8 1:/# nth_nbytes_flatten // LenNBytes.valP /#.
 qed.
 
 lemma pk_from_sig_correct (_msg_ _pub_seed_ : W8.t Array32.t, a1 a2 : W32.t Array8.t) :
@@ -613,11 +613,11 @@ conseq (: _ ==>
     + auto => /> ????addrL pkL pkR ?? H.
       rewrite /DecodeWotsPk.
       rewrite tP => j?.
-      by rewrite get_of_list // insubdK /P // H.
+      by rewrite get_of_list // LenNBytes.insubdK /P // H.
  
 seq 1 1 : (
-  val M{2} = to_list msg{1} /\
-  val _seed{2} = to_list pub_seed{1} /\
+  NBytes.val M{2} = to_list msg{1} /\
+  NBytes.val _seed{2} = to_list pub_seed{1} /\
   sig{2} = EncodeWotsSignature (load_sig Glob.mem{1} sig_ptr{1}) /\
 
   size tmp_pk{2} = 67 /\
@@ -627,11 +627,8 @@ seq 1 1 : (
 
   valid_ptr_i sig_ptr{1} XMSS_WOTS_SIG_BYTES 
 ).
-    + auto => /> *; do split.
-         * by rewrite insubdK // /P n_val size_to_list.
-         * by rewrite insubdK // /P n_val size_to_list.
-         * by rewrite size_nseq len_val.
-         *    
+    + by auto => /> *; rewrite size_nseq (: max 0 len = len) 1:/# len_val //= !NBytes.insubdK /P ?size_to_list ?n_val.
+
 seq 1 8 : (
     #pre /\ 
     map W32.to_uint (to_list lengths{1}) = msg{2} /\
@@ -774,8 +771,8 @@ while (
   0 <= i{1} <= len /\
   ={i} /\
   map W32.to_uint (to_list lengths{1}) = msg{2} /\
-  val M{2} = to_list msg{1} /\
-  val _seed{2} = to_list pub_seed{1} /\
+  NBytes.val M{2} = to_list msg{1} /\
+  NBytes.val _seed{2} = to_list pub_seed{1} /\
   sig{2} = EncodeWotsSignature (load_sig Glob.mem{1} sig_ptr{1}) /\
   size tmp_pk{2} = 67 /\
   valid_ptr_i sig_ptr{1} XMSS_WOTS_SIG_BYTES /\
@@ -818,15 +815,15 @@ seq 2 0 : (#pre /\ to_uint steps{1} = w - 1 - msg_i{2}).
 
 seq 2 0 : (#pre /\ to_uint t{1} = to_uint sig_ptr{1} + 32 * i{1}); first by auto => /> *; smt(@W64 pow2_64).     
 
-seq 1 1 : (#pre /\ to_list aux_0{1} = val sig_i{2}).
+seq 1 1 : (#pre /\ to_list aux{1} = NBytes.val sig_i{2}).
 - ecall {1} (p_memcpy_ptr_correct t{1}).
   auto => /> &1 &2 *; do split; 1..3: by smt().
   move => ???.
-  apply (eq_from_nth witness); rewrite ?valP size_to_list ?n_val // => j?.
-  rewrite get_to_list initiE //=  /EncodeWotsSignature /load_sig insubdK.
+  apply (eq_from_nth witness); rewrite ?NBytes.valP size_to_list ?n_val // => j?.
+  rewrite get_to_list initiE //=  /EncodeWotsSignature /load_sig LenNBytes.insubdK.
     + rewrite /P size_map size_chunk // size_to_list /#. 
   rewrite (nth_map witness); first by rewrite size_chunk // size_to_list /#.
-  rewrite insubdK.
+  rewrite NBytes.insubdK.
     + rewrite /P /chunk nth_mkseq /=; first by rewrite size_to_list /#.
       rewrite size_take // size_drop 1:/# size_to_list /#. 
   rewrite /chunk nth_mkseq.
@@ -843,8 +840,8 @@ call (gen_chain_correct P0 P1 P2 P3 P4 P5) => [/# |].
 auto => /> &1 &2 H0 H1 H2 H3 H4 H5 H6 H7 H8 H9 H10 H11 H12 H13 H14 H15 H16.
 rewrite size_map size_to_list in H10.
 do split.
-- apply nbytes_eq; apply (eq_from_nth witness); rewrite !valP ?n_val // => j?.
-  rewrite insubdK; first by rewrite /P size_to_list n_val.
+- apply nbytes_eq; apply (eq_from_nth witness); rewrite !NBytes.valP ?n_val // => j?.
+  rewrite NBytes.insubdK; first by rewrite /P size_to_list n_val.
   rewrite get_to_list initiE // /= initiE 1:/# /= ifT 1:/# -get_to_list H16.
   do congr => /#. 
 - smt().
@@ -921,11 +918,11 @@ conseq ( :
   sub addr{1} 0 5 = sub a1 0 5 /\
   sub addr{1} 0 5 = sub address{2} 0 5 /\
   M{2} = to_list msg{1} /\
-  val sk_seed{2} = to_list seed{1} /\ 
-  val pub_seed{2} = to_list pub_seed{1}
+  NBytes.val sk_seed{2} = to_list seed{1} /\ 
+  NBytes.val pub_seed{2} = to_list pub_seed{1}
   ==>
   _
-); first by auto => />; rewrite !insubdK // /P size_to_list n_val.
+); first by auto => />; rewrite !NBytes.insubdK // /P size_to_list n_val.
 
 seq 1 1 : (#pre /\ size sig{2} = len); first by auto => /> *; rewrite size_nseq len_val.
 
@@ -1069,8 +1066,8 @@ while (
     0 <= i{1} <= 67 /\
     ={i} /\
     size sig{2} = len /\
-    val sk_seed{2} = to_list seed{1} /\
-    val pub_seed{2} = to_list pub_seed{1} /\
+    NBytes.val sk_seed{2} = to_list seed{1} /\
+    NBytes.val pub_seed{2} = to_list pub_seed{1} /\
     M{2} = to_list msg{1} /\ 
 
     sub addr{1} 0 5 = sub address{2} 0 5 /\
@@ -1094,12 +1091,12 @@ while (
           rewrite H9 len_val => j?.
           rewrite (nth_map witness); first by rewrite size_chunk 1:/# size_to_list /#.
           apply nbytes_eq. 
-          rewrite insubdK. 
+          rewrite NBytes.insubdK. 
               * rewrite /P /chunk nth_mkseq /=; first by rewrite size_to_list /#.
                 rewrite size_take 1:/# size_drop 1:/# size_to_list /#.
           rewrite /chunk nth_mkseq /=; first by rewrite size_to_list.
-          apply (eq_from_nth witness); first by rewrite valP size_take 1:/# size_drop 1:/# size_to_list /#.
-          rewrite valP n_val => jj?.
+          apply (eq_from_nth witness); first by rewrite NBytes.valP size_take 1:/# size_drop 1:/# size_to_list /#.
+          rewrite NBytes.valP n_val => jj?.
           rewrite nth_take 1,2:/# nth_drop 1,2:/# get_to_list.
           have ->: sigL.[32*j + jj] = nth witness (sub sigL 0 (32 * iR)) (32*j + jj) by rewrite nth_sub // /#.
           rewrite H12 /sub_list nth_mkseq 1:/# /= nth_nbytes_flatten /#.
@@ -1128,12 +1125,12 @@ call (gen_chain_correct _P1 _P2 _P3 _P4 _P5 _P6) => [/# |].
 skip => /> &1 &2 H0 H1 H2 H3 H4 H5 H6 H7 H8 H9 H10 H11 H12 *.
 do split.
           + apply nbytes_eq.
-            rewrite insubdK /=; first by rewrite /P size_to_list /#.
-            apply (eq_from_nth witness); first by rewrite valP size_to_list /#.
-            rewrite valP n_val => j?.
+            rewrite NBytes.insubdK /=; first by rewrite /P size_to_list /#.
+            apply (eq_from_nth witness); first by rewrite NBytes.valP size_to_list /#.
+            rewrite NBytes.valP n_val => j?.
             rewrite get_to_list /= initiE //=.
             have ->: sig{1}.[i{2} * 32 + j] = nth witness (sub sig{1} (32 * i{2}) (2144 - 32 * i{2})) j by rewrite nth_sub /#.
-            rewrite H9 /DecodeWotsSk nth_sub 1:/# get_of_list 1:/# nth_nbytes_flatten 2:/# valP /#.
+            rewrite H9 /DecodeWotsSk nth_sub 1:/# get_of_list 1:/# nth_nbytes_flatten 2:/# LenNBytes.valP /#.
           + rewrite (nth_map witness); [by rewrite size_to_list | by rewrite get_to_list].
           + rewrite -H4 #smt:(@NBytes).
           + smt().
@@ -1169,9 +1166,9 @@ do split.
                  rewrite nth_sub 1:/# /DecodeWotsSk.
                  case (i{2} * 32 <= 32 * (i{2} + 1) + j && 32 * (i{2} + 1) + j < i{2} * 32 + 32) => //= H.
                     * rewrite get_of_list 1:/# nth_nbytes_flatten /#.
-                    * rewrite get_of_list 1:/# nth_nbytes_flatten; first by rewrite valP /#.
+                    * rewrite get_of_list 1:/# nth_nbytes_flatten; first by rewrite LenNBytes.valP /#.
                       have ->: sig{1}.[32 * (i{2} + 1) + j] = nth witness (sub sig{1} (32 * i{2}) (2144 - 32 * i{2})) (32 + j) by rewrite nth_sub /#.
-                      rewrite H9 nth_sub 1:/# /DecodeWotsSk get_of_list 1:/# nth_nbytes_flatten 2:/# valP /#.
+                      rewrite H9 nth_sub 1:/# /DecodeWotsSk get_of_list 1:/# nth_nbytes_flatten 2:/# LenNBytes.valP /#.
                * smt().
                * smt().
 qed.
