proof/correctness/SignProof.ec
@@ -193,7 +193,7 @@ seq 1 0 : (#pre /\ to_list idx_bytes{1} = EncodeIdx sk{2}.`idx).
    apply (eq_from_nth witness); first by rewrite size_EncodeIdx /XMSS_INDEX_BYTES size_to_list.
    rewrite size_to_list => j?.
    rewrite get_to_list initiE // /DecodeSkNoOID get_of_list 1:/#.
-   do 3! (rewrite nth_cat !size_cat size_EncodeIdx /XMSS_INDEX_BYTES !valP n_val ifT 1:/#).
+   do 3! (rewrite nth_cat !size_cat size_EncodeIdx /XMSS_INDEX_BYTES !NBytes.valP n_val ifT 1:/#).
    by rewrite nth_cat size_EncodeIdx /XMSS_INDEX_BYTES ifT 1:/#.
 
 seq 1 0 : (#pre /\ to_uint idx{1} = to_uint sk{2}.`Types.idx).
@@ -311,34 +311,34 @@ seq 1 1 : (
            case (0 <= j < 3) => ?.
               * rewrite (: aux_0{1}.[j] = nth witness (to_list aux_0{1}) j) 1:/# H27.
                 rewrite /DecodeSkNoOID get_of_list // => />.
-                do 3! (rewrite nth_cat !size_cat size_EncodeIdx /XMSS_INDEX_BYTES !valP n_val /= ifT 1:/#).
+                do 3! (rewrite nth_cat !size_cat size_EncodeIdx /XMSS_INDEX_BYTES !NBytes.valP n_val /= ifT 1:/#).
                 by rewrite nth_cat size_EncodeIdx /XMSS_INDEX_BYTES ifT 1:/#.
               * rewrite /DecodeSkNoOID get_of_list // => />.
                 rewrite get_of_list //. 
                 case (3 <= j < 3 + n) => ?.
-                  - do 3! (rewrite nth_cat !size_cat size_EncodeIdx /XMSS_INDEX_BYTES !valP n_val /= ifT 1:/#).
+                  - do 3! (rewrite nth_cat !size_cat size_EncodeIdx /XMSS_INDEX_BYTES !NBytes.valP n_val /= ifT 1:/#).
                     rewrite nth_cat size_EncodeIdx /XMSS_INDEX_BYTES ifF 1:/#.
-                    do 3! (rewrite nth_cat !size_cat size_EncodeIdx /XMSS_INDEX_BYTES !valP n_val /= ifT 1:/#).
+                    do 3! (rewrite nth_cat !size_cat size_EncodeIdx /XMSS_INDEX_BYTES !NBytes.valP n_val /= ifT 1:/#).
                     by rewrite nth_cat size_EncodeIdx /XMSS_INDEX_BYTES ifF 1:/#.
                 case (3 <= j < 3 + n + n ) => ?.
-                  - rewrite nth_cat !size_cat size_EncodeIdx /XMSS_INDEX_BYTES !valP n_val /= ifT 1:/#.
-                    rewrite nth_cat !size_cat size_EncodeIdx /XMSS_INDEX_BYTES !valP n_val /= ifT 1:/#.
-                    rewrite nth_cat !size_cat size_EncodeIdx /XMSS_INDEX_BYTES !valP n_val /= ifF 1:/#.
-                    rewrite nth_cat !size_cat size_EncodeIdx /XMSS_INDEX_BYTES !valP n_val /= ifT 1:/#.
-                    rewrite nth_cat !size_cat size_EncodeIdx /XMSS_INDEX_BYTES !valP n_val /= ifT 1:/#.
-                    by rewrite nth_cat !size_cat size_EncodeIdx /XMSS_INDEX_BYTES !valP n_val /= ifF 1:/#.                   
+                  - rewrite nth_cat !size_cat size_EncodeIdx /XMSS_INDEX_BYTES !NBytes.valP n_val /= ifT 1:/#.
+                    rewrite nth_cat !size_cat size_EncodeIdx /XMSS_INDEX_BYTES !NBytes.valP n_val /= ifT 1:/#.
+                    rewrite nth_cat !size_cat size_EncodeIdx /XMSS_INDEX_BYTES !NBytes.valP n_val /= ifF 1:/#.
+                    rewrite nth_cat !size_cat size_EncodeIdx /XMSS_INDEX_BYTES !NBytes.valP n_val /= ifT 1:/#.
+                    rewrite nth_cat !size_cat size_EncodeIdx /XMSS_INDEX_BYTES !NBytes.valP n_val /= ifT 1:/#.
+                    by rewrite nth_cat !size_cat size_EncodeIdx /XMSS_INDEX_BYTES !NBytes.valP n_val /= ifF 1:/#.                   
                 case (3 <= j < 3 + n + n + n) => ?.
-                  - rewrite nth_cat !size_cat size_EncodeIdx /XMSS_INDEX_BYTES !valP n_val /= ifT 1:/#.
-                    rewrite nth_cat !size_cat size_EncodeIdx /XMSS_INDEX_BYTES !valP n_val /= ifF 1:/#.
-                    rewrite nth_cat !size_cat size_EncodeIdx /XMSS_INDEX_BYTES !valP n_val /= ifT 1:/#.
-                    by rewrite nth_cat !size_cat size_EncodeIdx /XMSS_INDEX_BYTES !valP n_val /= ifF 1:/#.
-                rewrite nth_cat !size_cat size_EncodeIdx /XMSS_INDEX_BYTES !valP n_val /= ifF 1:/#.
-                rewrite nth_cat !size_cat size_EncodeIdx /XMSS_INDEX_BYTES !valP n_val /= ifF 1:/#.
+                  - rewrite nth_cat !size_cat size_EncodeIdx /XMSS_INDEX_BYTES !NBytes.valP n_val /= ifT 1:/#.
+                    rewrite nth_cat !size_cat size_EncodeIdx /XMSS_INDEX_BYTES !NBytes.valP n_val /= ifF 1:/#.
+                    rewrite nth_cat !size_cat size_EncodeIdx /XMSS_INDEX_BYTES !NBytes.valP n_val /= ifT 1:/#.
+                    by rewrite nth_cat !size_cat size_EncodeIdx /XMSS_INDEX_BYTES !NBytes.valP n_val /= ifF 1:/#.
+                rewrite nth_cat !size_cat size_EncodeIdx /XMSS_INDEX_BYTES !NBytes.valP n_val /= ifF 1:/#.
+                rewrite nth_cat !size_cat size_EncodeIdx /XMSS_INDEX_BYTES !NBytes.valP n_val /= ifF 1:/#.
                 reflexivity.
 
 seq 1 1 : (
     #pre /\ 
-    to_list index_bytes{1} = val idx_bytes{2} /\
+    to_list index_bytes{1} = NBytes.val idx_bytes{2} /\
     to_list index_bytes{1} = toByte idx{2} n 
 ).
     + ecall {1} (ull_to_bytes_32_correct idx{1}).
@@ -359,9 +359,9 @@ seq 1 1 : (
             congr; rewrite H28 EncodeIdxK2 //.
             rewrite /XMSS_FULL_HEIGHT /=; smt(@W32 pow2_32).
 
-      apply (eq_from_nth witness); first by rewrite valP n_val /toByte size_rev size_mkseq 1:/# /#. 
+      apply (eq_from_nth witness); first by rewrite NBytes.valP n_val /toByte size_rev size_mkseq 1:/# /#. 
       rewrite size_W64toBytes_ext // => j?.
-      rewrite insubdK; first by rewrite /P size_rev size_mkseq /#.
+      rewrite NBytes.insubdK; first by rewrite /P size_rev size_mkseq /#.
       rewrite toByte_32_64 1:/#.
       congr.
       rewrite -toByte_32_64 1:/# n_val.
@@ -375,18 +375,18 @@ seq 1 1 : (
  
 seq 1 0 : (
     #pre /\ 
-    to_list sk_prf{1} = val sk_prf{2}
+    to_list sk_prf{1} = NBytes.val sk_prf{2}
 ).
-    + auto => /> &1 &2 *; apply (eq_from_nth witness); rewrite ?valP ?n_val size_to_list // => j?.
+    + auto => /> &1 &2 *; apply (eq_from_nth witness); rewrite ?NBytes.valP ?n_val size_to_list // => j?.
       rewrite get_to_list initiE 1:/# /= /DecodeSkNoOID get_of_list 1:/#.
-      rewrite nth_cat !size_cat size_EncodeIdx /XMSS_INDEX_BYTES !valP n_val /= ifT 1:/#.
-      rewrite nth_cat !size_cat size_EncodeIdx /XMSS_INDEX_BYTES !valP n_val /= ifT 1:/#.
-      rewrite nth_cat !size_cat size_EncodeIdx /XMSS_INDEX_BYTES !valP n_val /= ifF 1:/#.
+      rewrite nth_cat !size_cat size_EncodeIdx /XMSS_INDEX_BYTES !NBytes.valP n_val /= ifT 1:/#.
+      rewrite nth_cat !size_cat size_EncodeIdx /XMSS_INDEX_BYTES !NBytes.valP n_val /= ifT 1:/#.
+      rewrite nth_cat !size_cat size_EncodeIdx /XMSS_INDEX_BYTES !NBytes.valP n_val /= ifF 1:/#.
       reflexivity.
 
 seq 1 1 : (
     #pre /\ 
-    to_list buf{1} = val _R{2}
+    to_list buf{1} = NBytes.val _R{2}
 ).
     + inline {1} M(Syscall).__prf_ M(Syscall)._prf; wp; sp; conseq />.      
       exists * in_00{1}, key0{1}; elim * => _P1 _P2.
@@ -394,13 +394,13 @@ seq 1 1 : (
       auto => /> &1 &2 H0 H1 H2 H3 H4 H5 H6 H7 H8 H9 H10 H11 H12 H13 H14 H15 H16 H17 H18 H19 H20 H21 H22 H23 H24 H25 H26 H27 H28 H29 H30 H31 *.
       do split; first by smt(@NBytes).
           - apply nbytes_eq.
-            rewrite insubdK; first by rewrite /P size_to_list /#.
-            apply (eq_from_nth witness); first by rewrite valP n_val size_to_list.
-            rewrite valP n_val => j?.
+            rewrite NBytes.insubdK; first by rewrite /P size_to_list /#.
+            apply (eq_from_nth witness); first by rewrite NBytes.valP n_val size_to_list.
+            rewrite NBytes.valP n_val => j?.
             by rewrite H31.
           - by move => ????->.
  
-seq 1 0 : (#pre /\ sub signature{1} XMSS_INDEX_BYTES n = val _R{2}).
+seq 1 0 : (#pre /\ sub signature{1} XMSS_INDEX_BYTES n = NBytes.val _R{2}).
     + auto => /> &1 &2 H0 H1 H2 H3 H4 H5 H6 H7 H8 H9 H10 H11 H12 H13 H14 H15 H16 H17 H18 H19 H20 H21 H22 H23 H24 H25 H26 H27 H28 H29 H30 H31 <-.
      do split; last first.
          * apply (eq_from_nth witness); first by rewrite size_to_list size_sub n_val.
@@ -419,20 +419,20 @@ seq 1 0 : (#pre /\ sub signature{1} XMSS_INDEX_BYTES n = val _R{2}).
  
 seq 1 0 : (
     #pre /\ 
-    to_list pub_root{1} = val root{2} 
+    to_list pub_root{1} = NBytes.val root{2} 
 ).
     + auto => /> &1 &2 H0 H1 H2 H3 H4 H5 H6 H7 H8 H9 H10 H11 H12 H13 H14 H15 H16 H17 H18 H19 H20 H21 H22 *.
-      apply (eq_from_nth witness); first by rewrite size_to_list valP n_val.
+      apply (eq_from_nth witness); first by rewrite size_to_list NBytes.valP n_val.
       rewrite size_to_list => i?.
       rewrite get_to_list initiE //=. 
       rewrite /DecodeSkNoOID get_of_list 1:/#.
-      rewrite nth_cat !size_cat size_EncodeIdx /XMSS_INDEX_BYTES !valP n_val ifT 1:/#.
-      rewrite nth_cat !size_cat size_EncodeIdx /XMSS_INDEX_BYTES !valP n_val ifF 1:/#.
+      rewrite nth_cat !size_cat size_EncodeIdx /XMSS_INDEX_BYTES !NBytes.valP n_val ifT 1:/#.
+      rewrite nth_cat !size_cat size_EncodeIdx /XMSS_INDEX_BYTES !NBytes.valP n_val ifF 1:/#.
       congr; ring.
  
 outline {2} [1-2] { 
     _M' <@ M_Hash.hash (
-          (insubd (val _R ++ val root ++ val idx_bytes))%ThreeNBytesBytes, 
+          (ThreeNBytesBytes.insubd (NBytes.val _R ++ NBytes.val root ++ NBytes.val idx_bytes))%ThreeNBytesBytes, 
           m); 
 }.
  
@@ -478,13 +478,13 @@ to_list aux_0{1} = EncodeIdx idx_new{2} /\
 1 <= to_uint sk{2}.`Types.idx <= 1048575 /\
 idx{2} = sk{2}.`Types.idx - W32.one /\
 to_uint idx{1} = to_uint sk{2}.`Types.idx - 1 /\
-to_list index_bytes{1} = val idx_bytes{2} /\
+to_list index_bytes{1} = NBytes.val idx_bytes{2} /\
 to_list index_bytes{1} = toByte idx{2} n /\
 
-to_list sk_prf{1} = val sk_prf{2} /\
-to_list buf{1} = val _R{2} /\
-sub signature{1} XMSS_INDEX_BYTES n = val _R{2} /\
-to_list pub_root{1} = val root{2} /\
+to_list sk_prf{1} = NBytes.val sk_prf{2} /\
+to_list buf{1} = NBytes.val _R{2} /\
+sub signature{1} XMSS_INDEX_BYTES n = NBytes.val _R{2} /\
+to_list pub_root{1} = NBytes.val root{2} /\
 
 to_uint t64{1} = to_uint sm_ptr{1} + (XMSS_SIG_BYTES - 128) /\
 sub signature{1} 0 XMSS_INDEX_BYTES = EncodeIdx idx{2}
@@ -524,15 +524,15 @@ seq 1 1 : (
   (1 <= to_uint sk{2}.`Types.idx && to_uint sk{2}.`Types.idx <= 1048575) /\
   idx{2} = sk{2}.`Types.idx - W32.one /\
   to_uint idx{1} = to_uint sk{2}.`Types.idx - 1 /\
-  to_list index_bytes{1} = val idx_bytes{2} /\
+  to_list index_bytes{1} = NBytes.val idx_bytes{2} /\
   to_list index_bytes{1} = toByte idx{2} n /\
-  to_list sk_prf{1} = val sk_prf{2} /\
-  to_list buf{1} = val _R{2} /\
-  sub signature{1} XMSS_INDEX_BYTES n = val _R{2} /\
-  to_list pub_root{1} = val root{2} /\
+  to_list sk_prf{1} = NBytes.val sk_prf{2} /\
+  to_list buf{1} = NBytes.val _R{2} /\
+  sub signature{1} XMSS_INDEX_BYTES n = NBytes.val _R{2} /\
+  to_list pub_root{1} = NBytes.val root{2} /\
 (* to_uint t64{1} = to_uint sm_ptr{1} + (XMSS_SIG_BYTES - 128) /\ *) 
 
-  to_list mhash{1} = val _M'{2} (* OBS: a partir daqui, o q ta em memoria nao me interessa *) /\
+  to_list mhash{1} = NBytes.val _M'{2} (* OBS: a partir daqui, o q ta em memoria nao me interessa *) /\
 
   address{2} = ots_addr{1} (* esqueci me disto *) /\
   idx_new{2} = sk{2}.`Types.idx /\
@@ -551,8 +551,8 @@ sub signature{1} 0 XMSS_INDEX_BYTES = EncodeIdx idx{2}
          * smt(@W64 pow2_64).
          * smt().
          * move => ?; rewrite /XMSS_FULL_HEIGHT /= /#.
-         * apply three_nbytes_eq; rewrite !insubdK.
-              - rewrite /P !size_cat !valP /#.
+         * apply three_nbytes_eq; rewrite !ThreeNBytesBytes.insubdK.
+              - rewrite /P !size_cat !NBytes.valP /#.
               - rewrite /P !size_cat !size_to_list size_toByte_64 /#. 
               - rewrite H29.
            do congr.
@@ -560,7 +560,7 @@ sub signature{1} 0 XMSS_INDEX_BYTES = EncodeIdx idx{2}
                 rewrite H27 get_to_list initiE //=. 
                 have ->: signature{1}.[3 + j] = nth witness (sub signature{1} XMSS_INDEX_BYTES n) j by rewrite nth_sub /#.
                 by rewrite H28.
-              - apply (eq_from_nth witness); rewrite valP n_val ?size_toByte_64 // => j?.
+              - apply (eq_from_nth witness); rewrite NBytes.valP n_val ?size_toByte_64 // => j?.
                 rewrite -H24 H25.
                 rewrite toByte_32_64 1:/#.
                 rewrite -W64toBytes_ext_toByte_64; congr; congr.
@@ -632,26 +632,26 @@ seq 1 1 : (
           rewrite size_to_list => j?; rewrite get_to_list nth_cat size_DecodeWotsSignature_List.
           case (0 <= j < n * len) => [Hfst | Hsnd]; [rewrite ifT 1:/# | rewrite ifF 1:/#].
              * rewrite /DecodeWotsSignature_List /EncodeWotsSignature.
-               rewrite nth_nbytes_flatten; first by rewrite valP /#.
+               rewrite nth_nbytes_flatten; first by rewrite LenNBytes.valP /#.
                rewrite /EncodeReducedSignature => />.
-               rewrite /EncodeWotsSignatureList insubdK.
+               rewrite /EncodeWotsSignatureList LenNBytes.insubdK.
                   + rewrite /P size_map size_chunk 1:/# size_sub_list /#.
                rewrite (nth_map witness). 
                   + rewrite size_chunk 1:/# size_sub_list /#.
-               rewrite insubdK.
+               rewrite NBytes.insubdK.
                   + rewrite /P nth_chunk 1:/#; first by rewrite size_sub_list /#.
                     rewrite size_take 1:/# size_drop 1:/# size_sub_list /#.
                rewrite nth_chunk 1:/#; first by rewrite size_sub_list /#.
                rewrite nth_take 1..2:/# nth_drop 1..2:/# nth_sub_list 1:/#.
                rewrite get_to_list /=; congr; smt().
              * rewrite /DecodeWotsSignature_List /EncodeWotsSignature.
-               rewrite nth_nbytes_flatten; first by rewrite valP /#.
+               rewrite nth_nbytes_flatten; first by rewrite AuthPath.valP /#.
                rewrite /EncodeReducedSignature => />.
-               rewrite /EncodeWotsSignatureList insubdK.
+               rewrite /EncodeWotsSignatureList AuthPath.insubdK.
                   + rewrite /P size_map size_chunk 1:/# size_sub_list /#.
                rewrite (nth_map witness). 
                   + rewrite size_chunk 1:/# size_sub_list /#.
-               rewrite insubdK.
+               rewrite NBytes.insubdK.
                   + rewrite /P nth_chunk 1:/#; first by rewrite size_sub_list /#.
                     rewrite size_take 1:/# size_drop 1:/# size_sub_list /#.
                rewrite nth_chunk 1:/#; first by rewrite size_sub_list /#.
@@ -677,7 +677,7 @@ seq 1 0 : (
            have ->: signature{1}.[j] = nth witness (sub signature{1} 0 XMSS_INDEX_BYTES) j by rewrite nth_sub /#.
            by rewrite H17 get_to_list.
 
-         - apply (eq_from_nth witness); first by rewrite valP size_sub /#.
+         - apply (eq_from_nth witness); first by rewrite NBytes.valP size_sub /#.
            rewrite n_val size_sub // => j?.
            rewrite nth_sub // initiE 1:/# /= ifF 1:/#. 
            rewrite -H27 nth_sub /#.
@@ -696,38 +696,38 @@ seq 0 1 : (
 ).
     + auto => /> &1 &2 H0 H1 H2 H3 H4 H5 H6 H7 H8 H9 H10 H11 H12 H13 H14 H15 H16 H17 H18 H19 H20 H21 H22 H23 H24 H25 H26 H27 H28 H29 H30 H31 H32 H33 H34 H35 H36 H37 H39.
       rewrite /EncodeReducedSignature; congr; [apply len_n_bytes_eq | apply  auth_path_eq].
-        - apply (eq_from_nth witness); first by rewrite !valP.
-          rewrite valP len_val => j?.
+        - apply (eq_from_nth witness); first by rewrite !LenNBytes.valP.
+          rewrite LenNBytes.valP len_val => j?.
           rewrite H39.
           apply nbytes_eq; apply (eq_from_nth witness); first by rewrite !NBytes.valP. 
-          rewrite valP n_val => k?.
-          rewrite /EncodeWotsSignatureList insubdK.
+          rewrite NBytes.valP n_val => k?.
+          rewrite /EncodeWotsSignatureList LenNBytes.insubdK.
              * rewrite /P size_map size_chunk // size_sub_list // /#. 
           rewrite (nth_map witness); first by rewrite size_chunk // size_sub_list // /#.
-          rewrite insubdK.
+          rewrite NBytes.insubdK.
              * rewrite /P /chunk nth_mkseq /=; first by rewrite size_sub_list /#. 
                rewrite size_take 1:/# size_drop 1:/# size_sub_list /#.
           rewrite nth_chunk 1:/#. 
              * rewrite size_sub_list /#.
           rewrite nth_take 1,2:/# nth_drop 1,2:/#.
           rewrite nth_sub_list 1:/# nth_cat size_DecodeWotsSignature_List ifT 1:/#.
-          rewrite /DecodeWotsSignature_List nth_nbytes_flatten 2:/# valP /#. 
-        - apply (eq_from_nth witness); first by rewrite !valP.
-          rewrite valP h_val d_val /= => j?.
+          rewrite /DecodeWotsSignature_List nth_nbytes_flatten 2:/# LenNBytes.valP /#. 
+        - apply (eq_from_nth witness); first by rewrite !AuthPath.valP.
+          rewrite AuthPath.valP h_val d_val /= => j?.
           rewrite H39.
           apply nbytes_eq; apply (eq_from_nth witness); first by rewrite !NBytes.valP. 
-          rewrite valP n_val => k?.
-          rewrite /EncodeWotsSignatureList insubdK.
+          rewrite NBytes.valP n_val => k?.
+          rewrite /EncodeWotsSignatureList AuthPath.insubdK.
              * rewrite /P size_map size_chunk 1:/# size_sub_list // /#. 
           rewrite (nth_map witness); first by rewrite size_chunk 1:/# size_sub_list /#.
-          rewrite insubdK.
+          rewrite NBytes.insubdK.
              * rewrite /P /chunk nth_mkseq /=; first by rewrite size_sub_list /#. 
                rewrite size_take 1:/# size_drop 1:/# size_sub_list /#.
           rewrite nth_chunk 1:/#. 
              * rewrite size_sub_list /#.
           rewrite nth_take 1,2:/# nth_drop 1,2:/#.
           rewrite nth_sub_list 1:/# nth_cat size_DecodeWotsSignature_List ifF 1:/#.
-          rewrite /DecodeWotsSignature_List nth_nbytes_flatten 2:/# valP /#. 
+          rewrite /DecodeWotsSignature_List nth_nbytes_flatten 2:/# AuthPath.valP /#. 
 
 seq 1 0 : (
   #{/~address{2} = ots_addr{1}}
@@ -766,10 +766,10 @@ while (
    1 <= to_uint sk{2}.`Types.idx <= 1048575 /\
    idx{2} = sk{2}.`Types.idx - W32.one /\
    to_uint idx{1} = to_uint sk{2}.`Types.idx - 1 /\
-   to_list index_bytes{1} = val idx_bytes{2} /\
+   to_list index_bytes{1} = NBytes.val idx_bytes{2} /\
    to_list index_bytes{1} = toByte idx{2} n /\
-   to_list sk_prf{1} = val sk_prf{2} /\
-   sub signature{1} XMSS_INDEX_BYTES n = val _R{2} /\
+   to_list sk_prf{1} = NBytes.val sk_prf{2} /\
+   sub signature{1} XMSS_INDEX_BYTES n = NBytes.val _R{2} /\
    to_uint idx_tree{1} = to_uint idx_tree{2} /\
    ={idx_leaf} /\
    0 <= to_uint idx_leaf{1} < 2 ^ 20 /\
@@ -785,7 +785,7 @@ while (
 
    1 <= j{2} <= 2 /\ i{1} = j{2} /\
    size (sig{2}.`r_sigs) = j{2}  /\
-   ((1 < i{1}) => to_list root{1} = val root{2}) /\
+   ((1 < i{1}) => to_list root{1} = NBytes.val root{2}) /\
 
    (forall (k : int), 0 <= k < size (sig{2}.`r_sigs) =>
      nth witness (sig{2}.`r_sigs) k = 
@@ -816,7 +816,7 @@ do split.
 
         * rewrite H46; apply nbytes_eq; rewrite -H42.    
           rewrite /EncodeSignature => />.
-          rewrite insubdK; first by rewrite /P size_sub_list /#.
+          rewrite NBytes.insubdK; first by rewrite /P size_sub_list /#.
           rewrite /XMSS_INDEX_BYTES /XMSS_N n_val.
           apply (eq_from_nth witness); rewrite size_sub // ?size_sub_list // => j?.
           by rewrite nth_sub // nth_sub_list // get_to_list.
@@ -859,17 +859,17 @@ do split.
 
 seq 2 0 : (
   #pre /\
-  to_list sk_seed{1} = val sk{2}.`Types.sk_seed /\
-  to_list pub_seed{1} = val sk{2}.`Types.pub_seed_sk
+  to_list sk_seed{1} = NBytes.val sk{2}.`Types.sk_seed /\
+  to_list pub_seed{1} = NBytes.val sk{2}.`Types.pub_seed_sk
 ).
     + auto => /> &1 &2 H0 H1 H2 H3 H4 H5 H6 H7 H8 H9 H10 H11 H12 H13 H14 H15 H16 H17 H18 H19 H20 H21 H22 H23 H24 H25 H26 H27 H28 H29 H30 H31 H32 H33 H34 H35 *.
-      do split; apply (eq_from_nth witness); rewrite size_to_list ?valP ?n_val // => j?; rewrite get_to_list initiE //= /DecodeSkNoOID get_of_list => />; 1,3: by smt().
-          - rewrite nth_cat !size_cat !valP n_val size_EncodeIdx /XMSS_INDEX_BYTES ifT 1:/#.
-            rewrite nth_cat !size_cat !valP n_val size_EncodeIdx /XMSS_INDEX_BYTES ifT 1:/#.  
-            rewrite nth_cat !size_cat !valP n_val size_EncodeIdx /XMSS_INDEX_BYTES ifT 1:/#.
+      do split; apply (eq_from_nth witness); rewrite size_to_list ?NBytes.valP ?n_val // => j?; rewrite get_to_list initiE //= /DecodeSkNoOID get_of_list => />; 1,3: by smt().
+          - rewrite nth_cat !size_cat !NBytes.valP n_val size_EncodeIdx /XMSS_INDEX_BYTES ifT 1:/#.
+            rewrite nth_cat !size_cat !NBytes.valP n_val size_EncodeIdx /XMSS_INDEX_BYTES ifT 1:/#.  
+            rewrite nth_cat !size_cat !NBytes.valP n_val size_EncodeIdx /XMSS_INDEX_BYTES ifT 1:/#.
             rewrite nth_cat size_EncodeIdx /XMSS_INDEX_BYTES ifF 1:/#.
             by [].
-          - rewrite nth_cat !size_cat !valP n_val size_EncodeIdx /XMSS_INDEX_BYTES ifF 1:/#.
+          - rewrite nth_cat !size_cat !NBytes.valP n_val size_EncodeIdx /XMSS_INDEX_BYTES ifF 1:/#.
             by [].
 
 seq 1 0 : (#pre /\ ots_addr{1}.[4] = W32.zero).
@@ -878,7 +878,7 @@ seq 1 0 : (#pre /\ ots_addr{1}.[4] = W32.zero).
 
 seq 1 1 : (
   #pre /\ 
-  to_list root{1} = val root{2}
+  to_list root{1} = NBytes.val root{2}
 ).
     + inline {1} 1; inline {1} 13.
       wp; conseq />.
@@ -932,26 +932,26 @@ seq 1 1 : (
           rewrite size_to_list => j?; rewrite get_to_list nth_cat size_DecodeWotsSignature_List.
           case (0 <= j < n * len) => [Hfst | Hsnd]; [rewrite ifT 1:/# | rewrite ifF 1:/#].
              * rewrite /DecodeWotsSignature_List /EncodeWotsSignature.
-               rewrite nth_nbytes_flatten; first by rewrite valP /#.
+               rewrite nth_nbytes_flatten; first by rewrite LenNBytes.valP /#.
                rewrite /EncodeReducedSignature => />.
-               rewrite /EncodeWotsSignatureList insubdK.
+               rewrite /EncodeWotsSignatureList LenNBytes.insubdK.
                   + rewrite /P size_map size_chunk 1:/# size_sub_list /#.
                rewrite (nth_map witness). 
                   + rewrite size_chunk 1:/# size_sub_list /#.
-               rewrite insubdK.
+               rewrite NBytes.insubdK.
                   + rewrite /P nth_chunk 1:/#; first by rewrite size_sub_list /#.
                     rewrite size_take 1:/# size_drop 1:/# size_sub_list /#.
                rewrite nth_chunk 1:/#; first by rewrite size_sub_list /#.
                rewrite nth_take 1..2:/# nth_drop 1..2:/# nth_sub_list 1:/#.
                rewrite get_to_list /=; congr; smt().
              * rewrite /DecodeWotsSignature_List /EncodeWotsSignature.
-               rewrite nth_nbytes_flatten; first by rewrite valP /#.
+               rewrite nth_nbytes_flatten; first by rewrite AuthPath.valP /#.
                rewrite /EncodeReducedSignature => />.
-               rewrite /EncodeWotsSignatureList insubdK.
+               rewrite /EncodeWotsSignatureList AuthPath.insubdK.
                   + rewrite /P size_map size_chunk 1:/# size_sub_list /#.
                rewrite (nth_map witness). 
                   + rewrite size_chunk 1:/# size_sub_list /#.
-               rewrite insubdK.
+               rewrite NBytes.insubdK.
                   + rewrite /P nth_chunk 1:/#; first by rewrite size_sub_list /#.
                     rewrite size_take 1:/# size_drop 1:/# size_sub_list /#.
                rewrite nth_chunk 1:/#; first by rewrite size_sub_list /#.
@@ -987,14 +987,14 @@ do split; 5,6,9,10: by smt().
       congr.
     + rewrite ifT 1:/#. 
       rewrite /EncodeReducedSignature; congr.
-        * apply len_n_bytes_eq; apply (eq_from_nth witness); rewrite !valP // len_val => i?.
-          rewrite /EncodeWotsSignatureList insubdK.
+        * apply len_n_bytes_eq; apply (eq_from_nth witness); rewrite !LenNBytes.valP // len_val => i?.
+          rewrite /EncodeWotsSignatureList LenNBytes.insubdK.
              - by rewrite /P size_map size_chunk // size_sub_list 1,2:/#.
           rewrite (nth_map witness); first by rewrite size_chunk // size_sub_list 1,2:/#.
           rewrite nth_chunk //; first by rewrite size_sub_list 1,2:/#.
           apply nbytes_eq.
-          apply (eq_from_nth witness); rewrite !valP // n_val => j?.
-          rewrite insubdK; first by rewrite /P size_take // size_drop 1:/# size_sub_list /#.
+          apply (eq_from_nth witness); rewrite !NBytes.valP // n_val => j?.
+          rewrite NBytes.insubdK; first by rewrite /P size_take // size_drop 1:/# size_sub_list /#.
           rewrite nth_take 1,2:/# nth_drop 1,2:/#.
           rewrite nth_sub_list 1:/# nth_sub 1:/# initiE 1:/# /=.
           rewrite ifT 1:/# /XMSS_INDEX_BYTES /=.
@@ -1002,17 +1002,16 @@ do split; 5,6,9,10: by smt().
                    nth witness (to_list aux_1{1}) (35 + k * 2464 + (32 * i + j) - (35 + size sig{2}.`r_sigs * 2464))
                    by rewrite get_to_list.
           rewrite H44 nth_cat size_DecodeWotsSignature_List ifT 1:/#.
-          rewrite /DecodeWotsSignature_List nth_nbytes_flatten; first by rewrite valP /#.
-          smt().
+          rewrite /DecodeWotsSignature_List nth_nbytes_flatten 2:/# LenNBytes.valP /#.
            
-        * apply auth_path_eq; apply (eq_from_nth witness); rewrite !valP // h_val d_val /= => i?.
-          rewrite /EncodeWotsSignatureList insubdK.
+        * apply auth_path_eq; apply (eq_from_nth witness); rewrite !AuthPath.valP // h_val d_val /= => i?.
+          rewrite /EncodeWotsSignatureList AuthPath.insubdK.
              - by rewrite /P size_map size_chunk 1:/# size_sub_list 1,2:/#.
           rewrite (nth_map witness); first by rewrite size_chunk 1:/# size_sub_list 1,2:/#.
           rewrite nth_chunk 1:/#; first by rewrite size_sub_list 1,2:/#.
           apply nbytes_eq.
-          apply (eq_from_nth witness); rewrite !valP // n_val => j?.
-          rewrite insubdK; first by rewrite /P size_take // size_drop 1:/# size_sub_list /#.
+          apply (eq_from_nth witness); rewrite !NBytes.valP // n_val => j?.
+          rewrite NBytes.insubdK; first by rewrite /P size_take // size_drop 1:/# size_sub_list /#.
           rewrite nth_take 1,2:/# nth_drop 1,2:/#.
           rewrite nth_sub_list 1:/# nth_sub 1:/# initiE 1:/# /=.
           rewrite ifT 1:/# /XMSS_INDEX_BYTES /=.
@@ -1022,6 +1021,6 @@ do split; 5,6,9,10: by smt().
           (35 + size sig{2}.`r_sigs * 2464))
                    by rewrite get_to_list.
           rewrite H44 nth_cat size_DecodeWotsSignature_List ifF 1:/#.
-          rewrite /DecodeWotsSignature_List nth_nbytes_flatten 2:/# valP /#.
+          rewrite /DecodeWotsSignature_List nth_nbytes_flatten 2:/# AuthPath.valP /#.
 qed.
 
