proof/spec/xmss_mt/XMSS_MT_PRF.ec
@@ -132,7 +132,7 @@ module XMSS_MT_PRF = {
       idx_bytes <- NBytes.insubd (toByte idx n);
       _R <@ Hash.prf(idx_bytes, sk_prf);
 
-      t <- ThreeNBytesBytes.insubd (val _R ++ val root ++ val idx_bytes); (* t = r || getRoot(SK_MT) || (toByte(idx_sig, n)) *)
+      t <- ThreeNBytesBytes.insubd (NBytes.val _R ++ NBytes.val root ++  NBytes.val idx_bytes); (* t = r || getRoot(SK_MT) || (toByte(idx_sig, n)) *)
       _M' <- H_msg t m;
 
       idx_tree <- idx `>>>` (h %/ d);
@@ -193,7 +193,7 @@ module XMSS_MT_PRF = {
        (* M' = H_msg(getR(Sig_MT) || getRoot(PK_MT) || (toByte(idx_sig, n)), M); *)
        root <- pk.`pk_root;
        _R <- s.`r;
-       t <- ThreeNBytesBytes.insubd (val _R ++ val root ++ val idx_bytes);
+       t <- ThreeNBytesBytes.insubd ( NBytes.val _R ++  NBytes.val root ++  NBytes.val idx_bytes);
        _M' <- H_msg t m; 
 
        address <- set_layer_addr address 0;
