proof/spec/xmss_mt/XMSS_MT_Types.ec
@@ -9,13 +9,11 @@ require import Types Array8 LTree.
 
 (******************************************************************************)
 
-clone export Subtype as AuthPath with
-  type T = nbytes list,
-  op P = fun l => size l = h %/ d (* Section 4.1.8. of the RFC *)
-                             (* The size is h / d for the multi tree variant *)
-  rename "sT" as "auth_path"
-  proof inhabited by (exists (nseq (h %/ d) (NBytes.insubd (nseq n W8.zero))); smt( size_nseq ge0_h ge0_d))
-  proof *.
+subtype auth_path as AuthPath = { l : nbytes list | size l = h %/ d }.
+realize inhabited.
+proof.
+by (exists (nseq (h %/ d) (NBytes.insubd (nseq n W8.zero))); smt( size_nseq ge0_h ge0_d)).
+qed.
 
 type sig_t = { sig_idx : W32.t;
                r : nbytes ;
